C0b

semantics.v
@@ -1,28 +1,87 @@
+Require Import String.
+Require Import List.
+Import ListNotations.
 Require Import syntax.
+Require Import util.
+
+Instance AddrTEq : EqDec AddrT.
+    constructor.
+    now repeat decide equality.
+Defined.
+Instance VarTEq : EqDec VarT.
+    constructor.
+    now repeat decide equality.
+Defined.
 
 Variant UndefVal :=
     | Undef
-    | Defined (v:Val)
-    .
+    | Defined (v:Val).
 
-Notation VarEnv := (VarT -> option AddrT).
-Notation MemEnv := (AddrT -> option UndefVal).
+Section Environments.
+    Variable (dom codom:Type).
+    Variable (DomEq : EqDec dom).
+
+    Definition Env := list (dom * codom).
+    Definition lookup (e:Env) a :=
+        r <- find (fun (d:dom * codom) => eqb (fst d) a) e;;
+        Some (snd r).
+
+    Fixpoint lookupStack (stack:list Env) (v:dom) :=
+        match stack with
+        | [] => None
+        | hd::tl =>
+            match lookup hd v with
+            | None => lookupStack tl v
+            | Some a => Some a
+            end
+        end.
+
+    (* needs list representation *)
+    Definition getCodom (e:Env) : list codom :=
+        map (fun (d:dom * codom) => snd d) e.
+    Definition getDom (e:Env) : list dom :=
+        map (fun (d:dom * codom) => fst d) e.
+
+    Definition undef (e:Env) (xs:list dom) : Env :=
+        filter (fun (d:dom * codom) =>
+            negb (mem (fst d) xs)) e.
+
+    Definition update (f:Env) (x:dom) (y:codom) :=
+        (x,y) :: f.
+    (* if @eqdec A Aeq x x2 then y else f x2. *)
+
+    Definition emptyEnv : Env := [].
+
+End Environments.
+
+Arguments lookup {dom} {codom} {DomEq}.
+Arguments lookupStack {dom} {codom} {DomEq}.
+Arguments undef {dom} {codom} {DomEq}.
+Arguments update {dom} {codom}.
+Arguments getDom {dom} {codom}.
+Arguments getCodom {dom} {codom}.
+Arguments emptyEnv {dom} {codom}.
+
+
+Notation VarEnv := (Env VarT AddrT).
+Notation MemEnv := (Env AddrT UndefVal).
 
 (* Record State :=
     {
         var_assign: VarEnv;
         memory_assign: MemEnv
     }. *)
-Definition State := (VarEnv * MemEnv)%type.
+Definition State := (list VarEnv * MemEnv)%type.
 
-Implicit Type (ρ:VarEnv) (μ:MemEnv) (σ:State).
+Implicit Type (ρ:VarEnv) (ρs:list VarEnv) (μ:MemEnv) (σ:State).
 
-Load option_monad.
+
+Definition ρmap σ := lookupStack (fst σ).
+Definition μmap σ := lookup (snd σ).
 
 Definition lookupVar σ x :=
-    let (ρ, μ) := σ in 
-    a <- ρ x;;
-    μ a.
+    a <- ρmap σ x;;
+    μmap σ a.
 
 Definition evalOp (op:Op) (v1 v2:Val) : option Val :=
     match op, v1,v2 with 
@@ -35,9 +94,9 @@ Definition evalOp (op:Op) (v1 v2:Val) : option Val :=
     end.
 
 Fixpoint LExprEval (l:LExpr) (σ:State) : option AddrT :=
-    let (ρ,μ) := σ in
     match l with
-    | Var x => ρ x
+    (* C0b *)
+    | Var x => ρmap σ x
     (* C0p *)
     | Indir e => 
         match RExprEval e σ with
@@ -49,9 +108,8 @@ with RExprEval (e:Expr) (σ:State) : option Val :=
     match e with 
     | Const c => ret c
     | LVal l => 
-        let (ρ,μ) := σ in
         a <- LExprEval l σ;;
-        uv <- μ a;;
+        uv <- μmap σ a;;
         match uv with 
         | Undef => None
         | Defined v =>
@@ -77,28 +135,11 @@ Variant Conf :=
     | Running (smt:Stmt) (s:State)
     .
 
-
-Class EqDec (A:Type) :=
-    {eqdec:(forall (x y:A), {x = y} + {x<>y})}.
-
-Definition update {A B} {Aeq:EqDec A} (f:A -> B) (x:A) (y:B) (x2:A) : B :=
-        if @eqdec A Aeq x x2 then y else f x2.
-
-Instance AddrTEq : EqDec AddrT.
-    constructor.
-    now decide equality.
-Defined.
-
-Instance StringEq : EqDec string.
-    constructor.
-    repeat decide equality.
-Defined.
-
-Notation RExprEval := ExprEval.
+Notation "f { x ↦ y }" := (update f x y) (at level 10).
 
 Notation "⟨ s | st ⟩" := (Running s st).
 Notation "« st »" := (Terminated st).
-Notation "R⟦ e ⟧ σ" := (ExprEval e σ) (at level 40).
+Notation "R⟦ e ⟧ σ" := (RExprEval e σ) (at level 40).
 Notation "L⟦ l ⟧ σ" := (LExprEval l σ) (at level 40).
 Notation "↯" := (Aborted).
 Coercion Terminated : State >-> Conf.
@@ -109,13 +150,38 @@ Coercion IntVal : nat >-> Val.
 Coercion Defined : Val >-> UndefVal.
 (* Coercion Some : UndefVal >-> (option UndefVal). *)
 
+Definition remove_codom {A B C} {BEq:EqDec B} (μ:Env B C) (ρ:Env A B) : Env B C :=
+    undef μ (getCodom ρ).
+
+Definition maxAddr μ :=
+    list_max(map (fun a =>
+        match a with
+        | NatAddr n => n
+        | _ => 0
+        end
+    ) (getDom μ)).
+
+Definition initAdresses μ xs v :=
+    fold_left
+    (fun e a =>
+        update e a v
+    ) xs μ.
+
+Definition getNewAdresses (decl:list Declaration) μ : VarEnv :=
+    let freshAddr := S(maxAddr μ) in
+    fold_left_i (fun e '(t,v) i =>
+        let a := NatAddr (i + freshAddr) in
+        e { v ↦ a }
+    ) decl emptyEnv.
+
+
 Reserved Notation "c1 ~> c2" (at level 50).
 Inductive step : Conf -> Conf -> Prop :=
-    | AssignStep l e ρ μ a v: 
-        let σ := (ρ, μ) in
+    | AssignStep l e ρs μ a v: 
+        let σ := (ρs, μ) in
         R⟦e⟧σ = Some v ->
         L⟦l⟧σ = Some a ->
-        ⟨ (Assign l e) | σ ⟩ ~> «(ρ, update μ a (Some (Defined v)))»
+        ⟨ (Assign l e) | σ ⟩ ~> «(ρs, update μ a (Defined v))»
     | IfTrueStep e s1 s2 σ (n:nat) :
         R⟦e⟧σ = Some (n:Val) ->
         n <> 0 ->
@@ -124,20 +190,34 @@ Inductive step : Conf -> Conf -> Prop :=
         R⟦e⟧σ = Some (0:Val) ->
         ⟨ (If e s1 s2) | σ ⟩ ~> ⟨ s2 | σ ⟩
     | WhileStep e s σ :
-        ⟨ (While e s) | σ ⟩ ~> ⟨ If e (Block [s; While e s]) (Block []) | σ ⟩
+        ⟨ (While e s) | σ ⟩ ~> ⟨ If e (Block [] [s; While e s]) (Block [] []) | σ ⟩
+    (* modified by C0b *)
     | EmptyStep σ :
-        ⟨ Block [] | σ ⟩ ~> « σ »
+        (* or ignore decls *)
+        ⟨ Block [] [] | σ ⟩ ~> « σ »
     | ExecStep s1 sr σ σ' :
         ⟨ s1 | σ ⟩ ~> « σ' » ->
-        ⟨ Block (s1::sr) | σ ⟩ ~> ⟨ Block sr | σ' ⟩
+        (* or ignore decls *)
+        ⟨ Block [] (s1::sr) | σ ⟩ ~> ⟨ Block [] sr | σ' ⟩
     | SubstStep s1 s1' sr σ σ' :
         ⟨ s1 | σ ⟩ ~> ⟨ s1' | σ' ⟩ ->
-        ⟨ Block (s1::sr) | σ ⟩ ~> ⟨ Block (s1'::sr) | σ' ⟩
+        (* or ignore decls *)
+        ⟨ Block [] (s1::sr) | σ ⟩ ~> ⟨ Block [] (s1'::sr) | σ' ⟩
     | AbortStep σ :
         ⟨ Abort | σ ⟩ ~> ↯
     | CrashStep s1 sr σ :
         ⟨ s1 | σ ⟩ ~> ↯ ->
-        ⟨ Block (s1::sr) | σ ⟩ ~> ↯
+        (* or ignore decls *)
+        ⟨ Block [] (s1::sr) | σ ⟩ ~> ↯
+    (* added by C0b *)
+    | BlockStep decl stmt ρs μ:
+        let ρ := getNewAdresses decl μ in
+        let addrs := getCodom ρ in
+        ⟨ Block decl stmt | (ρs,μ) ⟩ ~> 
+        ⟨ Block [] (stmt++[■]) | (ρ::ρs, initAdresses μ addrs Undef) ⟩
+    | LeaveStep ρ ρs μ:
+        ⟨ Block [] [■] | (ρ::ρs, μ) ⟩  ~>
+        « (ρs,remove_codom μ ρ) »
     where "c1 ~> c2" := (step c1 c2).
 
 Inductive trace : list Conf -> Prop :=
