util.v
@@ -1,0 +1,61 @@
+Require Import String.
+Require Import List.
+
+
+Arguments Some [A] _.
+Arguments None {A}.
+
+Definition ret {A : Type} (x : A) := Some x.
+ 
+Definition bind {A B : Type} (a : option A) (f : A -> option B) : option B :=
+  match a with
+    | Some x => f x
+    | None => None
+  end.
+
+Notation "A >>= F" := (bind A F) (at level 42, left associativity).
+
+Notation "X <- A ;; B" := (bind A (fun X => B)) 
+    (at level 61, A at next level, right associativity).
+
+Lemma mon_left_id : forall (A B : Type) (a : A) (f : A -> option B),
+  ret a >>= f = f a.
+intros.
+reflexivity.
+Qed.
+ 
+Lemma mon_right_id : forall (A : Type) (a : option A),
+  a >>= ret = a.
+intros.
+induction a; repeat reflexivity.
+Qed.
+ 
+Lemma mon_assoc :
+  forall (A B C : Type) (a : option A) (f : A -> option B) (g : B -> option C),
+    (a >>= f) >>= g = a >>= (fun (x:A) => f x >>= g).
+intros.
+induction a; repeat reflexivity.
+Qed.
+
+
+
+
+
+
+Class EqDec (A:Type) :=
+    {eqdec:(forall (x y:A), {x = y} + {x<>y})}.
+
+Definition eqb {A} {H:EqDec A} (x y : A) : bool :=
+  if @eqdec A H x y then true else false.
+
+Instance StringEq : EqDec string.
+    constructor.
+    repeat decide equality.
+Defined.
+
+(* or use find *)
+Definition mem {A} {AEq:EqDec A} (a:A) (xs:list A) := 
+    existsb (fun x => eqb x a) xs.
+
+Definition fold_left_i {A B:Type} (f: A -> B -> nat -> A) (xs:list B) (a:A) : A :=
+    fst (fold_left (fun '(a,i) b => (f a b i, S i) ) xs (a,0)).
